MicroPolicies/Instance.v
@@ -31,12 +31,12 @@ Definition ratom := (atom (mword mt) value_tag).
 Definition matom := (atom (mword mt) mem_tag).
 
 (* Machine initialisation *)
-Definition reg0 : {fmap reg mt -> ratom } :=
+Definition reg0 {sp:Symbolic.params} (Other: (Symbolic.tag_type Symbolic.ttypes Symbolic.R)) : {fmap reg mt -> atom (mword mt) (Symbolic.tag_type Symbolic.ttypes Symbolic.R) } :=
   [fmap (as_word 0, Atom (as_word 0) Other)
       ; (as_word 1, Atom (as_word 0) Other)
       ; (as_word 2, Atom (as_word 0) Other)
       ; (as_word 3, Atom (as_word 0) Other)
-      ; (as_word 4, Atom (as_word 0) Other)
+      ; (as_word 4, Atom (as_word (Nat.pow 2 15)) Other)
       ; (as_word 5, Atom (as_word 0) Other)
       ; (as_word 6, Atom (as_word 0) Other)
       ; (as_word 7, Atom (as_word 0) Other)
@@ -46,9 +46,17 @@ Definition reg0 : {fmap reg mt -> ratom } :=
       ; (as_word 19, Atom (as_word 0) Other)].
 
 
-Definition load (start : {fmap mword mt -> matom } * nat) nc : state :=
+Definition load {sp} {Other} {start_tag} {start_internal} (start : {fmap mword mt -> _ } * nat) nc : @Symbolic.state mt sp :=
   {| Symbolic.mem := fst start ;
-     Symbolic.regs := reg0 ;
-     Symbolic.pc := {| vala := word.as_word (snd start) ; taga := Level 0 |} ;
-     Symbolic.internal := tt ;
+     Symbolic.regs := reg0 Other;
+     Symbolic.pc := {| vala := word.as_word (snd start) ; taga := start_tag |} ;
+     Symbolic.internal := start_internal ;
      Symbolic.comp_num := nc|}.
+
+
+Require Import Merged.
+
+Definition step_eval_mp := (@Exec.stepf mt ops sym_lrc Merged.table_lrc).
+Definition step_eval_me := (@Exec.stepf mt ops Merged.sym_lrc_merged Merged.table).
+Definition step_mp := (@Symbolic.step mt ops sym_lrc Merged.table_lrc).
+Definition step_me := (@Symbolic.step mt ops Merged.sym_lrc_merged Merged.table).
