MicroPolicies/Merged.v
@@ -19,9 +19,12 @@ Unset Strict Implicit.
 Unset Printing Implicit Defensive.
 Import DoNotation.
 
+Export Symbolic.
 
 Section WithClasses.
 
+Notation sp := sym_lrc.
+  
 Context {mt : machine_types} {ops : machine_ops mt}.
 
 (* system call registers *)
@@ -92,132 +95,7 @@ end.
 
 Notation pc_type := (atom (tag_type Symbolic.P)).
 
-Record state := State {
-                    mem : memory;
-                    regs : registers;
-                    pc : pc_type;
-                    comp_num : nat (* smallest n such that number of components < 2^n *)
-}.
-
-Notation state_ev := (state * option event)%type.
-
-Inductive update :=
-  | RegWrite : (register + sys_reg) -> word -> update
-  | RegRead  : (register + sys_reg) -> update
-  | MemWrite : word -> word -> update
-  | MemRead : word -> update
-.
-
-
 Definition code := (seq (instr * mem_tag)).
-
-Local Notation "x .+1" := (x + 1).
-
-Definition executing (cde : code) (pc : mword mt) tg (i : instr) : Prop :=
- nth_error cde (nat_of_word pc) = Some (i,tg).
-
-
-Definition outputs := Symbolic.outputs.
-Definition inputs := outputs.
-
-Record ovec (op : opcode) : Type := OVec {
-  trpc : tag_type Symbolic.P;
-  tr   : hseq (tag_type) (outputs op);
-  }.
-
-Record ivec (op : opcode) : Type := IVec {
-  tpc : tag_type Symbolic.P;
-  ti  : tag_type Symbolic.M;
-  ts  : hseq tag_type (inputs op)
-}.
-
-
-Context {instr_rules : Z ->
-       forall op : opcode,
-       tag_type Symbolic.P ->
-       tag_type Symbolic.M ->
-       hseq (fun tk : Symbolic.tag_kind => tag_type tk) (inputs op) -> option (tag_type Symbolic.M) -> option (ovec op * option event)}.
-
-Definition next_state (st : state)
-  (op : opcode)
-  (iv : ivec op)
-  (* (op : instr)
-  (tpc : tag_type Symbolic.P)
-  (ti  : tag_type Symbolic.M)
-  (ts : hseq (tag_type) (inputs op)) *)
-  (tni : option (tag_type Symbolic.M)) (* tni is the tag of the potential new pointer *)
-  (k : ((ovec op) * (option event)) -> option state_ev) : option state_ev :=
-  do! i <-  (regs st 1);
-  do! i <- Some (Symbolic.convert (word.int_of_word (vala i)));
-  do! ov <- instr_rules i (tpc iv) (ti iv) (ts iv) tni; (* i is the content of RCOM register - used in ECall/ERet events *)
-    k ov.
-
-
-Definition next_state_do_update (st : state) (tk : Symbolic.tag_kind)
-           (tag : tag_type tk)
-           (updt : update) : option state := 
-  match tk, tag with
-  | Symbolic.R, t => match updt with
-        | RegWrite r x =>  let regs':= setm (regs st) (to_nat_bis r) (x@t) in
-                          Some (State (mem st) regs' (pc st) (comp_num st))
-        | RegRead r => do! a <- regs st (to_nat_bis r);
-                      let regs' := setm (regs st) (to_nat_bis r) (vala a)@t in
-                      Some (State (mem st) regs' (pc st) (comp_num st))
-        | _ => None
-        end
-  | Symbolic.M, t => match updt with
-        | MemWrite w1 w2 => let mem':= setm (mem st) w1 w2@t in
-                           Some (State mem' (regs st) (pc st) (comp_num st))
-        | MemRead w => do! a <- mem st w;
-                      let mem' := setm (mem st) w (vala a)@t in
-                      Some (State mem' (regs st) (pc st) (comp_num st))
-        | _ => None
-        end
-  | Symbolic.P, t => None
-  end.
-
-Fixpoint next_state_do_updates (st : state) (tks : seq Symbolic.tag_kind)
-         (tags : hseq (tag_type) tks)
-         (updts : seq update) : option state :=
-  match tks, tags with
-    | [:: ], _ => Some st
-    | [:: tk & tks' ], tags =>
-        do! updt <- ohead updts;
-        do! st' <- next_state_do_update st (hshead tags) updt;
-        next_state_do_updates st' (hsbehead tags) (behead updts)
-  end.
-
-(* pc' is the new, target pc *)
-Definition next_state_updates_and_pc (cde : code) (st : state) 
-  (op : opcode)
-  (iv : ivec op)
-  (updts : seq update)
-  (pc' : word) : option state_ev :=
-  let tni := match ((nth_error cde (nat_of_word pc'))) with | None => None | Some (_,t) => Some (t) end in
-  let k :=
-    (fun (ov_ev:((ovec op) * (option event))) => let (ov,ev) := ov_ev in
-       do! st' <- next_state_do_updates st (tr ov) updts;
-       Some (State (mem st') (regs st') pc'@(trpc ov) (comp_num st), ev)
-    ) in
-  next_state st iv tni k.
-
-Definition next_state_updates (cde : code) (st : state) 
-  (op : opcode)
-  (iv : ivec op)
-  (updts : seq update) : option state_ev :=
-  next_state_updates_and_pc cde st iv updts (word_of_nat (nat_of_word (vala (pc st))).+1).
-
-Fixpoint find_label_aux (cde : code) (l : label) (n : nat) : option nat :=
-  match cde with
-  | nil => None
-  | cons (MrLabel l2, _) ccde => if (eqn l l2) then (Some n) else find_label_aux ccde l (n+1)
-  | cons _ ccde => find_label_aux ccde l (n+1)
-  end.
-
-(* TODO : check for potential off-by-one error *)
-(* find the word w of a pc pointing to the label l in cde *)
-Definition find_label (cde : code) (l : label) : option nat :=
-  find_label_aux cde l 0.
 
 Definition binop_of_binop (b : binop) : Types.binop :=
   match b with
@@ -228,434 +106,9 @@ Definition binop_of_binop (b : binop) : Types.binop :=
   | Leq => LEQ
   end.
 
-(* allows to split memory between components *)
-Definition component_memory_prefix {k} (c : nat) (nc : nat) :=
- @word.shlw k (word_of_nat (c)) (word_of_nat ((word_size mt) - nc)). (* left shift *)
-
-Definition alloc_fun (cde : code) (st : state) : option state :=
-  do! ra_val <- regs st (to_nat R_RA);
-  let next_pc := (vala ra_val)@(taga (pc st)) in
-  do! current_instr <- nth_error cde (nat_of_word (vala (pc st)));
-  let current_c := (color (snd current_instr)) in
-  let prefix := (component_memory_prefix (1 + current_c) (comp_num st)) in
-  let mask := (component_memory_prefix ((2 ^ (comp_num st))-1) (comp_num st)) in
-  let prefix_filter := (fun mw => ((word.andw mw mask) == prefix) ) in (* keep only words starting with exactly prefix *)
-  (* TL TODO: Rely on the fact that it set implem is a sorted list, kinda fishy *)
-  let max_addr := last (prefix) (filter prefix_filter (domm (mem st))) in
-  (* create the new bloc *)
-  let atom : matom := (word.as_word (ssrint.Posz 0))@(def_mem_tag current_c false) in
-  do! size <- regs st (to_nat_bis (inr R_SC_ARG1));
-  do! length <- match word.int_of_word (vala size) with
-                | ssrint.Posz x => Some x
-                | ssrint.Negz _ => None
-                end;
-  let bloc :=
-      mkseq (fun n => ((word.addw max_addr (word.as_word (ssrint.Posz (n + 2)))), atom)) (* this + 2 is giving you one unallocated word between each block *)
-            length in
-  let mem' := unionm (mem st) (mkfmap bloc) in
-  (* return *)
-  do! addr <- (do! x <- hd_error bloc;
-                 Some (fst x));
-  let regs' := setm (regs st) (to_nat_bis (inr R_SC_RET)) addr@Other in
-  Some (State mem' regs' next_pc (comp_num st)).
-
-
 Definition alloc_label := 2 ^ 14.
 
-
-Definition reg_clear_read :=
-  let reg_list : seq nat := O :: 2 :: 3 :: 5 :: 6 :: 7 :: 16 :: 17 :: 18 :: 19 :: nil in
-  map (fun n => (RegRead (from_nat_bis n))) reg_list.
-
-(* return an hseq containing the tags of all registers apart from RA and RCOM, plus top_reg *)
-Definition reg_clear_list (regs : registers)
-  top_reg_tag : (hseq (Symbolic.tag_type lrc_tags) (inputs JUMP)) :=
-  let reg_list : seq nat := O :: 2 :: 3 :: 5 :: 6 :: 7 :: 16 :: 17 :: 18 :: 19 :: nil in
-  @Symbolic.make_hseq _ _ _ (top_reg_tag :: (map (fun n =>
-                                odflt top_reg_tag (omap taga (regs n))) reg_list)).
-
-(*** step / eval_step ***)
-
-Inductive step (cde : code) (st st' : state) (ev : option event) : Prop :=
-| step_nop : forall mem reg pc tpc ti nc
-    (ST   : st = State mem reg pc@tpc nc)
-    (INST : executing cde pc ti MrNop),
-    let mvec : ivec NOP := IVec tpc ti ([hseq] : hseq _ (inputs NOP)) in forall
-    (NEXT : next_state_updates cde st mvec [:: ] = Some (st', ev)),    step cde st st' ev
-| step_label : forall mem reg pc tpc ti l nc
-    (ST   : st = State mem reg pc@tpc nc)
-    (INST : executing cde pc ti (MrLabel l)),
-    let mvec : ivec NOP := IVec tpc ti ([hseq] : hseq _ (inputs NOP)) in forall
-    (NEXT : next_state_updates cde st mvec [:: ] = Some (st', ev)),    step cde st st' ev
-| step_const : forall mem reg pc tpc ti n r old (told : tag_type Symbolic.R) nc
-    (ST   : st = State mem reg pc@tpc nc)
-    (INST : executing cde pc ti (MrConst n r))
-    (OLD  : reg (to_nat r) = Some old@told),
-    let mvec := IVec tpc ti ([hseq told] : hseq _ (inputs CONST)) in forall
-    (NEXT : next_state_updates cde st mvec [:: RegWrite (inl r) (swcast n)] = Some (st', ev)),   step cde st st' ev
-| step_mov : forall mem reg pc tpc ti r1 w1 t1 r2 old told nc
-    (ST   : st = State mem reg pc@tpc nc)
-    (INST : executing cde pc ti (MrMov r1 r2))
-    (R1W  : reg (to_nat_bis r1) = Some w1@t1)
-    (OLD  : reg (to_nat_bis r2) = Some old@told),
-    let mvec := IVec tpc ti ([hseq t1; told] : hseq _ (inputs MOV)) in forall
-    (NEXT : next_state_updates cde st mvec [:: RegRead r1 ; RegWrite r2 w1 ] = Some (st', ev)),   step cde st st' ev
-| step_binop : forall mem reg pc tpc ti op r1 r2 r3 w1 w2 t1 t2 old told nc
-    (ST   : st = State mem reg pc@tpc nc)
-    (INST : executing cde pc ti (MrBinop op r1 r2 r3))
-    (R1W  : reg (to_nat r1) = Some w1@t1)
-    (R2W  : reg (to_nat r2) = Some w2@t2)
-    (OLD  : reg (to_nat r3) = Some old@told),
-    let mvec := IVec tpc ti ([hseq t1; t2; told] : hseq _ (inputs (BINOP (binop_of_binop op)))) in forall
-    (NEXT : next_state_updates cde st mvec [:: RegRead (inl r1) ; RegRead (inl r2) ; RegWrite (inl r3) (binop_denote (binop_of_binop op) w1 w2) ] = Some (st', ev)),
-      step cde st st' ev
-| step_load : forall mem reg pc tpc ti r1 r2 w1 w2 t1 t2 old told nc
-    (ST   : st = State mem reg pc@tpc nc)
-    (INST : executing cde pc ti (MrLoad r1 r2))
-    (R1W  : reg (to_nat r1) = Some w1@t1)
-    (MEM1 : mem w1 = Some w2@t2)
-    (OLD  : reg (to_nat r2) = Some old@told),
-    let mvec := IVec tpc ti ([hseq t1; t2; told] : hseq _ (inputs LOAD)) in forall
-    (NEXT : next_state_updates cde st mvec [:: RegRead (inl r1) ; MemRead w1 ; RegWrite (inl r2) w2 ] = Some (st', ev)),
-    step cde st st' ev
-| step_store : forall mem reg pc r1 r2 w1 w2 tpc ti t1 t2 old told nc
-    (ST   : st = State mem reg pc@tpc nc)
-    (INST : executing cde pc ti (MrStore r1 r2))
-    (R1W  : reg (to_nat r1) = Some w1@t1)
-    (R2W  : reg (to_nat r2) = Some w2@t2)
-    (OLD  : mem w1 = Some old@told),
-    let mvec := IVec tpc ti ([hseq t1; t2; told] : hseq _ (inputs STORE)) in forall
-    (NEXT : next_state_updates cde st mvec [:: RegRead (inl r1) ; RegRead (inl r2) ; MemWrite w1 w2 ] = Some (st', ev)),
-    step cde st st' ev
-| step_jump : forall mem reg pc r w tpc ti t1 nc
-    (ST   : st = State mem reg pc@tpc nc)
-    (INST : executing cde pc ti (MrJump r))
-    (RW   : reg (to_nat r) = Some w@t1),
-    let mvec := IVec tpc ti ((reg_clear_list reg t1) : hseq _ (inputs JUMP)) in forall
-    (NEXT : next_state_updates_and_pc cde st mvec ((RegRead (inl r)) :: reg_clear_read) w = Some (st', ev)),
-    step cde st st' ev
-| step_bnz : forall mem reg pc r n w tpc ti t1 nc
-    (ST   : st = State mem reg pc@tpc nc)
-    (INST : executing cde pc ti (MrBnz r n))
-    (RW   : reg (to_nat r) = Some w@t1),
-    let mvec := IVec tpc ti ([hseq t1] : hseq _ (inputs BNZ)) in
-    let optpc' := (if w == (word_of_nat 0) then Some ((nat_of_word (pc)) + 1) else find_label cde n) in forall pc' (PC' : optpc' = Some pc')
-    (NEXT : next_state_updates_and_pc cde st mvec [:: RegRead (inl r) ] (word_of_nat pc') = Some (st', ev)),
-    step cde st st' ev
-| step_jal : forall mem reg pc l tpc ti old told pc' nc
-    (ST : st = State mem reg pc@tpc nc)
-    (INST : executing cde pc ti (MrJal l))
-    (OLD : reg (to_nat R_RA) = Some old@told)
-    (NOT_ALLOC : l <> alloc_label),
-    let mvec := IVec tpc ti ((reg_clear_list reg told) : hseq _ (inputs JAL)) in
-    forall (PC' :  Some pc' = (find_label cde l))
-      (NEXT : next_state_updates_and_pc cde st mvec
-                ((RegWrite (inl R_RA) (word_of_nat((nat_of_word pc).+1))) :: reg_clear_read) (word_of_nat pc') = Some (st', ev)),
-    step cde st st' ev
-| step_jal_alloc : forall mem reg pc  l tpc ti old told st_inter nc
-    (ST : st = State mem reg pc@tpc nc)
-    (INST : executing cde pc ti (MrJal l))
-    (OLD : reg (to_nat R_RA) = Some old@told)
-    (ALLOC : l = alloc_label),
-    forall (NEXT : @next_state_do_update st Symbolic.R Other ( RegWrite (inl R_RA) (word_of_nat((nat_of_word pc).+1))) = Some st_inter)
-    (ST' : (alloc_fun cde st_inter) = Some st') (EV : ev = None),
-    step cde st st' ev
-.
-
-
-Definition eval_step (cde : code) (st : state) : option state_ev := 
-  let 'State mem reg pc@pctag nc := st in
-  match (nth_error cde (nat_of_word pc)) with
-  | None =>None
-  | Some (instr,ti) =>
-    match instr with
-    | MrNop | MrLabel _ =>
-      let mvec := IVec pctag ti ([hseq] : hseq _ (inputs NOP)) in
-      next_state_updates cde st mvec [:: ]
-    | MrConst n r =>
-      do! old <- reg (to_nat r);
-      let: _@told := old in
-      let ivec := IVec pctag ti ([hseq told] : hseq _ (inputs CONST)) in
-      next_state_updates cde st ivec [:: RegWrite (inl r) (swcast n)]
-    | MrMov r1 r2 =>
-      do! a1 <- reg (to_nat_bis r1);
-      let: w1@t1 := a1 in
-      do! a2 <- (reg (to_nat_bis r2));
-      let: _@told := a2 in
-      let mvec := IVec pctag ti ([hseq t1;told] : hseq _ (inputs MOV)) in
-      next_state_updates cde st mvec [:: RegRead r1 ; RegWrite r2 w1]
-    | MrBinop op r1 r2 r3 =>
-      do! a1 <- reg (to_nat r1);
-      let: w1@t1 := a1 in
-      do! a2 <- reg (to_nat r2);
-      let: w2@t2 := a2 in
-      do! a3 <- reg (to_nat r3);
-      let: _@told := a3 in
-      let mvec := IVec pctag ti ([hseq t1;t2;told] : hseq _ (inputs (BINOP (binop_of_binop op)))) in
-      next_state_updates cde st mvec [:: RegRead (inl r1) ; RegRead (inl r2) ; RegWrite (inl r3) (binop_denote (binop_of_binop op) w1 w2)]
-    | MrLoad r1 r2 =>
-      do! a1 <- reg (to_nat r1);
-      let: w1@t1 := a1 in
-      do! amem <- mem w1;
-      let: w2@t2 := amem in
-      do! a2 <- reg (to_nat r2);
-      let: _@told := a2 in
-      let mvec := IVec pctag ti ([hseq t1;t2;told] : hseq _ (inputs LOAD)) in
-      next_state_updates cde st mvec [:: RegRead (inl r1) ; MemRead w1 ; RegWrite (inl r2) w2]
-    | MrStore r1 r2 =>
-      do! a1 <- reg (to_nat r1);
-      let: w1@t1 := a1 in
-      do! amem <- mem w1;
-      let: _@told := amem in
-      do! a2 <- reg (to_nat r2);
-      let: w2@t2 := a2 in
-      let mvec := IVec pctag ti ([hseq t1;t2;told] : hseq _ (inputs STORE)) in
-      next_state_updates cde st mvec [:: RegRead (inl r1) ; RegRead (inl r2) ; MemWrite w1 w2]
-    | MrJump r =>
-      do! a <- reg (to_nat r);
-      let: w@t1 := a in
-      let mvec := IVec pctag ti ((reg_clear_list reg t1) : hseq _ (inputs JUMP)) in
-      next_state_updates_and_pc cde st mvec ((RegRead (inl r)) :: reg_clear_read) w
-    | MrBnz r n =>
-      do! a <- reg (to_nat r);
-      let: w@t1 := a in
-      do! pc' <- (if w == (word_of_nat 0) then Some ((nat_of_word (pc)) + 1) else find_label cde n);
-      let ivec := IVec pctag ti ([hseq t1] : hseq _ (inputs BNZ)) in
-      next_state_updates_and_pc cde st ivec [:: RegRead (inl r)] (word_of_nat pc')
-    | MrJal i =>
-        do! oldtold <- reg (to_nat R_RA);
-        let: _@told := oldtold in
-        if (i == alloc_label) then
-        do! st_inter <- (@next_state_do_update st Symbolic.R Other ( RegWrite (inl R_RA) (word_of_nat((nat_of_word pc).+1))));
-        do! st' <- alloc_fun cde st_inter;
-        Some (st', None)
-      else
-        let mvec := IVec pctag ti ((reg_clear_list reg told) : hseq _ (inputs JAL)) in
-        match (find_label cde i) with
-        | None => None
-        | Some (pc') => next_state_updates_and_pc cde st mvec
-                         ((RegWrite (inl R_RA) (word_of_nat((nat_of_word pc).+1))) :: reg_clear_read) (word_of_nat pc')
-        end
-    | MrHalt => None
-    end
-  end.
-
-
-Lemma eq_op_to_eq : forall (x y : nat), (x = y) <-> (true = (x == y)).
-Proof.
-  intro x.
-  induction x ; split ; intro eq ; try ( induction y ; try reflexivity ; inversion eq ).
-  + unfold "==", nat_eqType, nat_eqMixin. simpl.
-    unfold "==", nat_eqType, nat_eqMixin in IHx.
-    remember (IHx y) as a. destruct a as [l r]. simpl in l. destruct Heqa. rewrite H0 in l.
-    apply l. reflexivity.
-  + cut (x=y).
-    ++ intro. auto.
-    ++ apply IHx. auto.
-Qed.
-
-
-Theorem eval_step_complete:
-  forall cd st st' ev, step cd st st' ev -> eval_step cd st = Some (st', ev).
-Proof.
-  intros. inversion H ;
-  try (unfold executing in INST ) ;
-  try (unfold eval_step ; rewrite ST ; rewrite INST ; rewrite <- ST ; unfold mvec in NEXT) ;
-  try (rewrite R1W) ; simpl ; try (rewrite R2W) ; simpl ; try (rewrite RW ) ; simpl ;
-  try (rewrite MEM1); simpl ; try (rewrite OLD) ; simpl ; try exact NEXT.
-  + unfold optpc' in PC'. rewrite PC'. auto.
-  + remember (l == alloc_label) as cond. induction cond ; try (rewrite <- PC' ; exact NEXT).
-    unfold "==", nat_eqType, nat_eqMixin in Heqcond; simpl.
-    inversion Heqcond as [eq]. destruct (@eqnP l alloc_label). destruct (NOT_ALLOC e). inversion eq.
-  +  unfold eval_step. rewrite ST.  rewrite INST. rewrite OLD. simpl. rewrite <- ALLOC.
-     rewrite <- (fst (eq_op_to_eq l l)) ; try reflexivity. rewrite EV. 
-    remember {|mem := mem0; regs := setm reg 4 (word_of_nat (nat_of_word pc0).+1)@Other;
-     pc := pc0@tpc0; comp_num := nc |} as st_alt. cut (st_alt = st_inter).
-    ++ intro eq. rewrite <- eq in ST'. rewrite Heqst_alt in ST'. rewrite ST'. auto.
-    ++ unfold next_state_do_update,to_nat_bis, to_nat in NEXT. rewrite ST in NEXT.
-       inversion NEXT. exact Heqst_alt.
-Qed.
-
-
-(* those tactics help when STEP_EQ contains something of the form  "do! _ <- regs0 (f s);" *)
-
-Ltac resolve_register regs0 STEP_EQ s f :=
-  let rval  := fresh in
-  remember (regs0 (f s)) as rval ; destruct rval ; simpl in STEP_EQ. 
-  
-Ltac resolve_register_deep regs0 STEP_EQ s f :=
-  let save  := fresh in 
-  let Heqsave := fresh in 
-  let rval  := fresh in 
-  let Heqrval := fresh in 
-       remember (regs0 (f s)) as save eqn:Heqsave ;
-       unfold Option.bind, oapp, getm in STEP_EQ ;
-       remember (getm_def regs0 (f s)) as rval eqn:Heqrval ;
-       cut (rval = save) ; try (rewrite Heqsave ; rewrite Heqrval ; reflexivity) ;
-       unfold getm_def in STEP_EQ ; unfold getm_def in Heqrval ;
-       simpl in Heqrval ; simpl in STEP_EQ ; rewrite <- Heqrval in STEP_EQ ; destruct rval.
-      (* +++ destruct a. intro tageq. rewrite <- tageq in Heqsave. *)
-
-
-Ltac resolve_memory_deep regs0 STEP_EQ s :=
-  let save  := fresh in 
-  let Heqsave := fresh in 
-  let rval  := fresh in 
-  let Heqrval := fresh in 
-       remember (regs0 s) as save eqn:Heqsave ;
-       unfold Option.bind, oapp, getm in STEP_EQ ;
-       remember (getm_def regs0 s) as rval eqn:Heqrval ;
-       cut (rval = save) ; try (rewrite Heqsave ; rewrite Heqrval ; reflexivity) ;
-       unfold getm_def in STEP_EQ ; unfold getm_def in Heqrval ;
-       simpl in Heqrval ; simpl in STEP_EQ ; rewrite <- Heqrval in STEP_EQ ; destruct rval.
-
-Theorem eval_step_sound:
-  forall cd st st' ev
-    (STEP_EQ : eval_step cd st = Some (st', ev)), step cd st st' ev.
-  intros. unfold eval_step in STEP_EQ.
-  induction st.  induction pc0 as [pcv pctag].
-  remember ({| mem := mem0; regs := regs0; pc := pcv@pctag |}) as st.
-  remember (nth_error cd (nat_of_word pcv)) as nth.
-  destruct nth as [iti|]. destruct iti as [i ti].
-  induction i.
-  + apply (step_nop Heqst (esym Heqnth) STEP_EQ). 
-  + apply (step_label Heqst (esym Heqnth) STEP_EQ). 
-  + remember (regs0 (to_nat r)) as rval. destruct rval ; simpl in STEP_EQ.
-    ++ destruct a as [old told].
-       apply (step_const Heqst (esym Heqnth) (esym Heqrval) STEP_EQ).
-    ++ inversion STEP_EQ.
-  + resolve_register regs0 STEP_EQ s to_nat_bis.
-    ++ destruct a as [old told]. resolve_register_deep regs0 STEP_EQ s0 to_nat_bis.
-       +++ destruct a as [old0 told0]. intro tageq. rewrite <- tageq in H0.
-           apply (step_mov Heqst (esym Heqnth) (esym HeqH) (esym H0) STEP_EQ). 
-       +++ inversion STEP_EQ. 
-    ++ inversion STEP_EQ.
-  + resolve_register regs0 STEP_EQ r to_nat.
-    ++ destruct a as [w1 t1]. resolve_register_deep regs0 STEP_EQ r0 to_nat.
-       +++ destruct a as [old0 told0]. intro tageq. rewrite <- tageq in H0.
-           resolve_register_deep regs0 STEP_EQ r1 to_nat.
-           ++++ destruct a as [old1 told1]. intro tageq1. rewrite <- tageq1 in H3.
-                apply (step_binop Heqst (esym Heqnth) (esym HeqH) (esym H0) (esym H3) STEP_EQ).
-           ++++ inversion STEP_EQ.
-       +++ inversion STEP_EQ.
-    ++ inversion STEP_EQ.
-  + resolve_register regs0 STEP_EQ r to_nat.
-    ++ destruct a as [w1 t1]. 
-       resolve_memory_deep mem0 STEP_EQ w1.
-       +++ destruct a as [old0 told0]. intro tageq. rewrite <- tageq in H0.
-           resolve_register_deep regs0 STEP_EQ r0 to_nat.
-           ++++ destruct a as [old1 told1]. intro tageq1. rewrite <- tageq1 in H3.
-                apply (step_load Heqst (esym Heqnth) (esym HeqH) (esym H0) (esym H3) STEP_EQ). 
-           ++++ inversion STEP_EQ.
-       +++ inversion STEP_EQ.
-    ++ inversion STEP_EQ.
-  + resolve_register regs0 STEP_EQ r to_nat.
-    ++ destruct a as [w1 t1]. 
-       resolve_register_deep regs0 STEP_EQ r0 to_nat.
-       +++ destruct a as [old0 told0]. intro tageq. rewrite <- tageq in H0.
-           resolve_memory_deep mem0 STEP_EQ w1.
-           ++++ destruct a as [old1 told1]. intro tageq1. rewrite <- tageq1 in H3.
-                apply (step_store Heqst (esym Heqnth) (esym HeqH) (esym H0) (esym H3) STEP_EQ).
-           ++++ inversion STEP_EQ.
-       +++ resolve_memory_deep mem0 STEP_EQ w1 ; try (destruct a) ; inversion STEP_EQ.
-    ++ inversion STEP_EQ.
-  + resolve_register regs0 STEP_EQ r to_nat.
-    ++ destruct a as [w1 t1]. 
-       apply (step_jump Heqst (esym Heqnth) (esym HeqH) STEP_EQ).
-    ++ inversion STEP_EQ.
-  + resolve_register regs0 STEP_EQ r to_nat.
-    ++ destruct a as [w1 t1].
-       remember (if w1 == word_of_nat 0 then Some (nat_of_word pcv).+1 else find_label cd l) as save.
-       unfold Option.bind, oapp, "==", nat_eqType, nat_eqMixin in STEP_EQ.
-       remember ((if Equality.op (Equality.class (word_eqType (word_size mt))) w1 (word_of_nat 0)
-               then Some (nat_of_word pcv).+1
-                  else find_label cd l)) as pc'.
-       cut (save = pc') ; try (rewrite Heqsave ; rewrite Heqpc' ; reflexivity). intro Heqif.
-       rewrite Heqsave in Heqif. destruct pc'.
-       +++ apply (step_bnz Heqst (esym Heqnth) (esym HeqH) (Heqif) STEP_EQ).
-       +++ inversion STEP_EQ.
-    ++ inversion STEP_EQ.
-  + remember (l == alloc_label) as cond. destruct cond.
-    (* l = alloc_label case *)
-    ++ remember (@next_state_do_update st Symbolic.R Other ( RegWrite (inl R_RA) (word_of_nat((nat_of_word pcv).+1)))) as st_inter. 
-       destruct st_inter ; simpl in STEP_EQ.
-       +++ remember (alloc_fun cd s) as st_final. destruct st_final; simpl in STEP_EQ.
-           ++++ resolve_memory_deep regs0 STEP_EQ 4.
-                * intro eqa. destruct a as [old told]. inversion STEP_EQ.
-                remember (regs0 (to_nat R_RA)) as rval. destruct rval.
-                **  destruct a. unfold "==", nat_eqType, nat_eqMixin in Heqcond; simpl.
-                    rewrite H3 in Heqst_final.
-                    inversion Heqcond as [eq]. destruct (@eqnP l alloc_label) as [alloceq|].
-                    *** apply (step_jal_alloc Heqst (esym Heqnth) (esym Heqrval) alloceq (esym Heqst_inter) (esym Heqst_final)). reflexivity.
-                    *** inversion eq.
-                **  rewrite <- eqa in H0. simpl in Heqrval.
-                    unfold getm, getm_def in H0, Heqrval. simpl in Heqrval, H0.
-                    rewrite <- Heqrval in H0. inversion H0.
-                * inversion STEP_EQ.
-           ++++ resolve_memory_deep regs0 STEP_EQ 4 ; (try destruct a) ; inversion STEP_EQ.
-       +++ resolve_memory_deep regs0 STEP_EQ 4 ; (try destruct a) ; inversion STEP_EQ.
-    (* l <> alloc_label case *)
-    ++ simpl in STEP_EQ. resolve_memory_deep regs0 STEP_EQ 4 ; intro eq.
-       +++ destruct a as [old told]. remember (find_label cd l) as pc'.
-           cut (l <> alloc_label).
-           ++++ intro ineq.
-                destruct pc' as [pc'|].
-                * rewrite H0 in eq. apply (step_jal Heqst (esym Heqnth) (esym eq) ineq Heqpc' STEP_EQ).
-                * inversion STEP_EQ.
-                  ++++ intro eql. remember (eq_op_to_eq l alloc_label) as equi.
-                       destruct equi as [limp rimp]. rewrite <- (limp eql) in Heqcond.
-                       inversion Heqcond.
-       +++ inversion STEP_EQ.
-    ++ inversion STEP_EQ.
-  + inversion STEP_EQ.
-Qed.
-
-Theorem eval_step_equiv_step:
-  forall cd st st' ev, (eval_step cd st = Some (st', ev)) <-> (step cd st st' ev).
-  intros.
-  split.
-  + apply eval_step_sound.
-  + apply eval_step_complete.
-Qed.
-
-
-Fixpoint execN (n: nat) (cde: code) (st: state) : option Z + nat :=
-  match n with
-  | O => inr 3
-  | S n' =>
-    match eval_step cde st with
-    | None => (inl (
-             do! w <- (regs st (to_nat R_COM));
-             Some (Symbolic.convert (word.int_of_word (vala w)))))
-    | Some (st', _) => execN n' cde st'
-    end
-  end.
-
-
-Fixpoint execN_trace (n: nat) (cde: code) (st: state) : trace :=
-  match n with
-  | O => []
-  | S n' =>
-    match eval_step cde st with
-    | None => []
-    | Some (st', None) => execN_trace n' cde st'
-    | Some (st', Some ev) => ev :: (execN_trace n' cde st')
-    end
-  end.
-
 (*** Tagged -> Merged ***)
-
-Fixpoint fold_left {A B : Type} (f : B -> A -> B) (init : B) (l : list A) : B :=
-  match l with
-  | nil => init
-  | cons e ll => fold_left f (f init e) ll
-end.
-
-Fixpoint fold_right {A B : Type} (f : B -> A -> B) (init : B) (l : list A) : B :=
-  match l with
-  | nil => init
-  | cons e ll => f (fold_right f init ll) e
-end.
 
 Fixpoint fold_left_map {FROM ACC TO: Type} (f : ACC -> FROM -> TO * ACC) (init : ACC) (l : list FROM) : list TO :=
   match l with
@@ -671,19 +124,11 @@ end.
 
 (* gives you the beginning point of each buffers in memory *)
 Definition memory_lengths (buf : NMap {fmap Block.id -> nat + seq value}):  NMap (NMap nat) :=
-  (*
-  (* this takes into account the fact that the allocation is linearized into 5 instructions *)
-  let size_instr := (fun (i:Transitional.instr) => match i with | TrAlloc _ _ => 5 | _ => 1 end) in
-  let size_sum := (fold_left (fun n im => n + 1) 0) in
-  let l := Maps.elementsm (mapm (fun m => mkfmap (size_sum (Maps.elementsm m))) buf) in
-  mkfmap (fold_left_map (fun (count : nat) (p:nat*nat) => let (color, size) := p in ((color,count), count+size)) 0 l).*)
-
   let l := Maps.elementsm (mapm Maps.elementsm buf) in (* turns fmaps into lists *)
   let f := (fun acc => fold_left_map_bis (fun acc' (a : nat * (nat + seq value)) =>
                                      match (snd a) with
                                       | inl n => ((fst a, acc'), n + acc')
-                                      | inr s => ((fst a, acc'), (size s) + acc') end
-                      ) acc) in
+                                      | inr s => ((fst a, acc'), (size s) + acc') end ) acc) in
   mkfmap (fold_left_map (fun acc s => let (flat,count) := f acc (snd s) in
                            ((fst s, mkfmap (flat)), count + acc) ) 0 l).
 
@@ -823,19 +268,19 @@ Definition initial_memory (p : Intermediate.program) :=
      taga := snd x |})
   in Tmp.mapk f (mapm (encode_memval) bufs).
 
-Definition reg0 : registers :=
-  let default_reg := (word_of_nat 0)@(LRC.Other): atom (tag_type Symbolic.R) in
-  [fmap (0, default_reg) ;
-   (1, default_reg) ;
-   (2, default_reg) ;
-   (3, default_reg) ;
-   (4, (word_of_nat (2 ^ 15))@(LRC.Other)) ; (* value equivalent to "Undef" for R_RA*)
-   (5, default_reg) ;
-   (6, default_reg) ;
-   (16,default_reg) ;
-   (17,default_reg) ;
-   (18,default_reg) ;
-   (19,default_reg) ].
+Definition reg0 : {fmap reg mt -> (@ratom mt) } :=
+  [fmap (word_of_nat 0, Atom (word_of_nat 0) Other)
+      ; (word_of_nat 1, Atom (word_of_nat 0) Other)
+      ; (word_of_nat 2, Atom (word_of_nat 0) Other)
+      ; (word_of_nat 3, Atom (word_of_nat 0) Other)
+      ; (word_of_nat 4, Atom (word_of_nat (2 ^ 15)) Other)
+      ; (word_of_nat 5, Atom (word_of_nat 0) Other)
+      ; (word_of_nat 6, Atom (word_of_nat 0) Other)
+      ; (word_of_nat 7, Atom (word_of_nat 0) Other)
+      ; (word_of_nat 16, Atom (word_of_nat 0) Other)
+      ; (word_of_nat 17, Atom (word_of_nat 0) Other)
+      ; (word_of_nat 18, Atom (word_of_nat 0) Other)
+      ; (word_of_nat 19, Atom (word_of_nat 0) Other)].
 
 
 (* return the memory along with the first pc *)
@@ -851,25 +296,12 @@ Definition encode_code_placeholder (cde : code) (pc0 : nat) : {fmap word_ordType
   Tmp.mapk (fun x => word_of_nat (x + pc0)) (fmap_of_seq (map (fun '(_,t) => Atom (word_of_nat 0) t) cde)).
  *)
 
-Definition initial_state cde (p : Intermediate.program) :=
+
+Definition initial_state cde (p : Intermediate.program) : (Symbolic.state sp) :=
   let nc := (1+ Nat.log2 (1 + (size (domm (Intermediate.prog_interface p))))) in
   let mem0 := (initial_memory p) in
   let pctag := build_tpc 0 in
-  {|mem := unionm (encode_code cde (size mem0)) mem0 ; regs := reg0 ; pc := (word_of_nat 0)@pctag ; comp_num := nc|}.
-
-Definition run_merged cd fuel p :=
-      execN fuel cd (initial_state cd p).
-
-
-Definition compile_run_merged fuel (p : Intermediate.program) :=
-  run_merged (transitional_to_merged p (intermediate_to_transitional p)) fuel p.
-
-Definition compile_and_run_from_source_merged := 
-fun (p : Source.program) (fuel : nat) =>
-match Compiler.compile_program p with
-| Some compiled_p => compile_run_merged fuel compiled_p
-| None => inl None
-end.
+  {|mem := unionm (encode_code cde (size mem0)) mem0 ; regs := reg0 ; pc := (word_of_nat 0)@pctag ; internal := tt; comp_num := nc|}.
 
 End WithClasses.
 
@@ -883,8 +315,7 @@ Definition instr_rules (rcom_val : Z)
   tpc
   ti
   (ts : hseq _ (inputs op))
-  tni
-  : option ((ovec op) * (option event)) :=
+  tni :=
   (* checks that we're not executing data *)
   do! _ <- match tni with
          | None => Some tt
@@ -910,7 +341,7 @@ Definition transfer (iv : Symbolic.ivec lrc_tags) (evi : Symbolic.ev_inputs) : o
   | Symbolic.IVec vop tpc ti ts tni =>
     match vop, ts, ti, tni return option (Symbolic.vovec _ vop * option event) with
     | (OP op), ts, ti, tni =>
-        do! out:(ovec op * option event) <- instr_rules (Symbolic.rcom_value evi) tpc ti ts tni;
+        do! out:((ovec _ op) * option event) <- instr_rules (Symbolic.rcom_value evi) tpc ti ts tni;
         let (ov, ev) := out in
         Some (Symbolic.OVec op (trpc ov) (tr ov), ev)
     (* Monitor stuff *)
@@ -929,7 +360,7 @@ Definition sym_lrc_merged : Symbolic.params := {|
 
 
 
-Definition lrc_alloc_fun (st : @Symbolic.state mt sym_lrc_merged) : option (Symbolic.state sym_lrc_merged) :=
+Definition alloc_fun (st : @Symbolic.state mt sym_lrc_merged) : option (Symbolic.state sym_lrc_merged) :=
   do! ra_val <- Symbolic.regs st ra;
   let next_pc := (vala ra_val)@(taga (Symbolic.pc st)) in
   (* TL TODO: Is using return address to compute calling component safe? *)
@@ -959,42 +390,11 @@ Definition lrc_alloc_fun (st : @Symbolic.state mt sym_lrc_merged) : option (Symb
 
 
 Definition table : (Symbolic.syscall_table sym_lrc_merged) :=
-  [fmap ((word_of_nat alloc_label), (@Symbolic.Syscall mt sym_lrc_merged tt lrc_alloc_fun ) )].
+  [fmap ((word_of_nat alloc_label), (@Symbolic.Syscall mt sym_lrc_merged tt alloc_fun ) )].
 
 
 Definition alloc_addr : imm mt := shlw 1%w (as_word (ssrint.Posz 14)). (* 1 << 14 ; as to be an imm for Jal, so under 2^15 *)
 Definition table_lrc : @Symbolic.syscall_table mt sym_lrc :=
   [fmap (swcast alloc_addr, {| Symbolic.entry_tag := tt ; Symbolic.sem := LRC.alloc_fun |})].
 
-Definition step_m := @step mt instr_rules.
-Definition step_s := (@Symbolic.step mt ops sym_lrc table_lrc).
-
-
-Inductive state_merged_equiv (s:@state mt) (s':@Symbolic.state mt sym_lrc) :=
-| State_merged_equiv_def :
-  ((@Symbolic.State mt sym_lrc) (mem s) (Tmp.mapk word_of_nat (regs s)) (pc s) tt (comp_num s)) = s' ->
-  state_merged_equiv s s'.
-
-Theorem step_equiv cde p s1 s2 s1' s2' ev:
-  cde = (transitional_to_merged p (intermediate_to_transitional p)) ->
-  state_merged_equiv s1  s2  ->
-  state_merged_equiv s1' s2' ->
-  ((step_m cde s1 s1' ev)) <-> ((step_s s2 s2' ev ))
-.
-Admitted.
-
-               
 End WithClasses'.
-
-Definition compile_and_run_from_source_merged_ex (mt : machine_types) {ops : machine_ops mt} := 
-fun (p : Source.program) (fuel : nat) =>
-match Compiler.compile_program p with
-| Some compiled_p =>
-    match @compile_run_merged mt ops instr_rules fuel compiled_p with
-    | inl (Some n) => print_ocaml_int (z2int n)
-    | inl None => print_error ocaml_int_1
-    | inr n => print_error (nat2int n)
-    end
-| None => print_error ocaml_int_0
-end.
-
